copy.v
@@ -1,67 +1,107 @@
-Require Import braun util.
-Require Import Arith.Even Arith.Div2 Omega.
+Require Import braun util monad fl_log.
+Require Import Arith Arith.Even Arith.Div2 Omega.
+Require Import Coq.Logic.JMeq Coq.Program.Wf.
+
 Set Implicit Arguments.
 
-Program Definition copy2 A (x:A) : forall n, braun_tree A (n+1) * braun_tree A n :=
-  Fix lt_wf _
-      (fun n copy2 =>
-         match n with
-           | 0 => (Node x 0 0 _ Empty Empty, Empty)
-           | S n' => 
-             match even_odd_dec n' with
-               (* odd *)
-               | right H =>
-                 let m := odd_S2n n' H
-                 in let (s, t) := copy2 (proj1_sig m) _
-                    in (Node x (m+1) (m+1) _ s s, Node x (m+1) m _ s t)
-               (* even *)
-               | left H =>
-                 let m := even_2n n' H 
-                 in let (s, t) := copy2 (proj1_sig m) _
-                    in (Node x (m+1) m _ s t, Node x m m _ t t)
-             end
-         end).
+Section copy2.
 
-Lemma odd_cleanup_1 : 
-  forall n, 
-    odd n -> div2 n + 1 + (div2 n + 1) + 1 = S (n + 1).
-  intros n H.
-  apply odd_double in H.
-  unfold double in H.
-  omega.
-Qed.
+  Variable A:Set.
+  Variable x:A.
 
-Lemma odd_cleanup_2 :
-  forall n,
-    odd n -> div2 n + 1 + div2 n + 1 = S n.
-  intros n H.
-  apply odd_double in H.
-  unfold double in H.
-  omega.
-Qed.
+  Program Definition helper_ss_st (m:nat) 
+          (pr : (braun_tree A (m+1) * (braun_tree A m)))
+  : C ((braun_tree A (m+m+3)) * (braun_tree A (m+m+2))) 2 :=
+    match pr with
+      | (s,t) =>
+        ( ++2 ;
+          ret (Node x (m+1) (m+1) _ s s,
+               Node x (m+1) m _ s t))
+    end.
+  
+  Solve Obligations using (intros ; omega).
 
-Lemma even_cleanup_1 : 
-  forall n,
-    even n -> div2 n + 1 + div2 n + 1 = S (n + 1).
-  intros n H.
-  apply even_double in H.
-  unfold double in H.
-  omega.
-Qed.
+  Program Definition helper_st_tt (m:nat) 
+          (pr : (braun_tree A (m+1) * (braun_tree A m)))
+  : C ((braun_tree A (m+m+2)) * (braun_tree A (m+m+1))) 2 :=
+    match pr with
+      | (s,t) =>
+        (++2 ;
+         ret (Node x (m+1) m _ s t,
+              Node x m m _ t t))
+    end.
 
-Lemma even_cleanup_2 :
-  forall n,
-    even n -> div2 n + div2 n + 1 = S n.
-  intros n H.
-  apply even_double in H.
-  unfold double in H.
-  omega.
-Qed.
+  Solve Obligations using (intros; omega).
 
-Solve Obligations using (intros; omega).
-Obligation 4. rewrite odd_cleanup_1. omega. assumption. Qed.
-Obligation 6. rewrite odd_cleanup_2. omega. assumption. Qed.
-Obligation 9. rewrite even_cleanup_1. omega. assumption. Qed.
-Obligation 11. rewrite even_cleanup_2. omega. assumption. Qed.
 
-Definition copy A (x:A) n := snd (copy2 x n).
+  Lemma odd_cleanup : 
+    forall k n, 
+      odd n -> div2 n + (div2 n) + (1+k) = n + k.
+    intros n k H.
+    apply odd_double in H.
+    unfold double in H.
+    omega.
+  Defined.
+
+  Lemma even_cleanup : 
+    forall k n,
+      even n -> div2 n + (div2 n) + k = n + k.
+    intros n k H.
+    apply even_double in H.
+    unfold double in H.
+    omega.
+  Defined.
+
+  Definition copy_rt n := S (2 * fl_log n).
+
+  Program Fixpoint copy2 (n:nat) {wf lt n}
+  : C ((braun_tree A (n+1)) * (braun_tree A n)) 
+      (copy_rt n) :=
+    match n with 
+      | 0 => (++1 ; ret (Node x 0 0 _ Empty Empty,Empty))
+      | S n' => 
+        match even_odd_dec n' with
+          | right H =>
+            p <- (copy2 (proj1_sig (odd_S2n n' H))) ;
+              helper_ss_st p
+          | left H =>
+            p <- (copy2 (proj1_sig (even_2n n' H))) ;
+              helper_st_tt p
+        end
+    end.
+
+  Obligation 3. rewrite (odd_cleanup 2). omega. assumption. Defined.
+  Obligation 4. rewrite (odd_cleanup 1). omega. assumption. Defined.
+
+  Obligation 7. rewrite (even_cleanup 2). omega. assumption. Defined.
+  Obligation 8. rewrite (even_cleanup 1). omega. assumption. Defined.
+
+  Obligation 5.
+    replace (fl_log (div2 n') + (fl_log (div2 n') + 0) + 2) 
+      with ((fl_log (div2 n') + 1) + (fl_log (div2 n') + 1)) ; [| omega].
+    rewrite fl_log_div2.
+    unfold copy_rt.
+    unfold mult.
+    rewrite plus_0_r.
+    reflexivity.
+  Qed.
+
+  Obligation 9.
+    replace (fl_log (div2 n') + (fl_log (div2 n') + 0) + 2) 
+    with ((fl_log (div2 n') + 1) + (fl_log (div2 n') + 1)) ; [| omega].
+    rewrite fl_log_div2.
+    unfold copy_rt.
+    unfold mult.
+    rewrite plus_0_r.
+    reflexivity.
+  Qed.
+
+  Program Definition copy n : C (braun_tree A n) (copy_rt n) :=
+    c <- (copy2 n) ;
+    match c with
+      | (t1,t2) => ret t2
+    end.
+
+  Solve Obligations using (intros; omega).
+
+End copy2.
