insert.v
@@ -1,13 +1,37 @@
-Require Import braun Omega Coq.Logic.JMeq.
 Set Implicit Arguments.
 
-Program Fixpoint insert A n (x:A)
-        (b : braun_tree A n)
-: braun_tree A (n+1) :=
+Require Import braun util monad fl_log.
+Require Import Coq.Logic.JMeq Coq.Program.Wf.
+Require Import Arith Arith.Even Arith.Div2.
+Require Import Omega.
+
+Program Fixpoint insert (A:Set) n (x:A) (b : braun_tree A n)
+: C (braun_tree A (n+1)) (fl_log n + 1) :=
   match b with
-    | Empty => Node x 0 0 _ Empty Empty
-    | Node y s_size t_size p s t => 
-      Node x (t_size+1) s_size _ (insert y t) s
+    | Empty =>
+      (++1 ;
+       ret (Node x 0 0 _ Empty Empty))
+    | Node y s_size t_size p s t =>
+      (st <- (insert y t);
+       ++ 1;
+       ret (Node x
+                 (t_size+1) s_size
+                 _
+                 st s))
   end.
 
 Solve Obligations using (intros;omega).
+
+Obligation 2.
+  assert (s_size = t_size \/ s_size = t_size + 1) as TwoCases;
+    [ omega | ].
+
+  inversion TwoCases; subst; clear.
+  
+  rewrite fl_log_odd.
+  reflexivity.
+
+  replace (t_size + 1 + t_size + 1) with ((t_size+1) + (t_size+1)); [| omega].
+  rewrite fl_log_even.
+  reflexivity.
+Qed.
