old/insert.v
@@ -1,0 +1,13 @@
+Require Import braun Omega Coq.Logic.JMeq.
+Set Implicit Arguments.
+
+Program Fixpoint insert A n (x:A)
+        (b : braun_tree A n)
+: braun_tree A (n+1) :=
+  match b with
+    | Empty => Node x 0 0 _ Empty Empty
+    | Node y s_size t_size p s t => 
+      Node x (t_size+1) s_size _ (insert y t) s
+  end.
+
+Solve Obligations using (intros;omega).
