old/monad.v
@@ -1,0 +1,69 @@
+(*
+Following the ideas from
+  Coq-Formalized Proofs of Quicksort's Average-case Complexity
+  By Eelis van der Weegen and James McKinna, TYPES 2008
+  paper:
+  http://github.com/Eelis/qs-avg/raw/f0535088e7f1b7d7fc0d5ac06867a09a1c282f94/papers/TYPES08/published.pdf
+
+  code: https://github.com/Eelis/qs-avg
+*)
+
+
+Set Implicit Arguments.
+
+Require Import Arith Omega Coq.Logic.JMeq.
+
+Definition C (s: Set): Set := (s * nat)%type. 
+
+Definition bind A B (xn: C A) (y: A -> C B): C B :=
+  match xn with
+    | (x,n) =>
+      match y x with
+        | (r,n') => (r,n+n')
+      end
+  end.
+Definition ret (A: Set) (x: A): C A := (x,0).
+
+Definition inc (A : Set) (k : nat) (x : C A) : C A :=
+  match x with
+    | (v,n) => (v, n+k)
+  end.
+
+Definition time := snd.
+
+Module MonadLaws.
+
+  (* (return x >>= f) = (f x) *)
+  Theorem mon_lunit: 
+    forall (a b: Set) (x: a)
+           (f: a -> C b), 
+      bind (ret x) f = f x.
+
+    intros; unfold bind; unfold ret.
+    destruct (f x).
+    simpl.
+    reflexivity.
+  Qed.
+
+  (* (f >>= return) = f *)
+  Theorem mon_runit: forall (a: Set) (f: C a), bind f (@ret a) = f.
+    intros; unfold bind; unfold ret.
+    destruct f.
+    rewrite plus_0_r; reflexivity.
+  Qed.
+
+  (* ((n >>= f) >>= g) = n >>= (\x -> f x >>= g) *)
+  Theorem mon_assoc: forall a b c (n: C a) (f: a -> C b) (g: b -> C c),
+      bind (bind n f) g =
+      bind n (fun x => bind (f x) g).
+    intros; unfold bind.
+    destruct n; destruct (f a0); destruct (g b0).
+    rewrite plus_assoc; reflexivity.
+  Qed.
+
+End MonadLaws.
+
+Notation "x >>= y" := (bind x y) (at level 55).
+Notation "x >> y" := (bind x (fun _ => y)) (at level 30, right associativity).
+Notation "x <- y ; z" := (bind y (fun x : _ => z)) (at level 30, right associativity).
+Notation "++ k ; c" := (inc k c) (at level 30, right associativity).
