size.v
@@ -1,103 +1,12 @@
 Require Import braun util monad.
-Require Import Coq.Logic.JMeq Coq.Program.Wf.
-Require Import Arith Arith.Even Arith.Div2.
-Require Import Omega.
-Require Import Program.Syntax.
 Set Implicit Arguments.
 
-(*size implemented with the implementation of braun_trees from braun.v*)
-
-(*size without monads*)
-Program Fixpoint size A n (b : braun_tree A n) : nat :=
+Program Fixpoint size_linear A n (b : braun_tree A n) : C nat n :=
   match b with
-    |Empty => 0
-    |Node y s_size t_size p s t => 
-     1 + size s + size t
+    | Empty => ret 0
+    | Node y s_size t_size p s t =>
+      (++ 1;
+       s_sz <- size_linear s;
+       t_sz <- size_linear t;
+       ret (s_sz + t_sz + 1))
   end.
-
-Program Example size_example1 :
-  size (Node 1 0 0 _ Empty Empty)
-       = 1.
-compute;reflexivity.
-
-Program Example size_example2 :
-  size (Node 1 2 1 _ 
-             (Node 2 1 0 _ 
-                   (Node 3 0 0 _ Empty Empty) 
-                   Empty)
-             (Node 4 0 0 _ Empty Empty))
-       = 4.
-compute;reflexivity.
-
-(*size done with counting monad*)
-Program Fixpoint sizem A n (b : braun_tree A n):
-  C (nat) :=
-  match b with
-    |Empty => ret 0
-    |Node y s_size t_size p s t =>
-     s_sz <- sizem s;
-       t_sz <- sizem t;
-       ++ 1;
-       ret (S (s_sz + t_sz))
-  end.
-
-Program Example sizem_ex1 :
-  time(sizem (Node 1 2 1 _ 
-                   (Node 2 1 0 _ 
-                         (Node 3 0 0 _ Empty Empty) 
-                         Empty)
-                   (Node 4 0 0 _ Empty Empty)))
-  =4.
-compute;reflexivity.
-
-Program Example sizem_ex2 :
-  fst(sizem (Node 1 2 1 _ 
-                  (Node 2 1 0 _ 
-                        (Node 3 0 0 _ Empty Empty) 
-                        Empty)
-                  (Node 4 0 0 _ Empty Empty)))
-  =4.
-compute;reflexivity.
-
-Theorem size_runtime_linear: forall (A:Set) n (x:A)
-                             (b : braun_tree A n),
-                        time (sizem b) = 
-                        fst (sizem b).
-  intros.
-  induction b;intros;simpl.
-  reflexivity.
-  unfold bind.
-  remember (sizem b2) as t eqn:TEQ.
-  destruct t.
-  remember (sizem b1) as t2 eqn:T2EQ.
-  destruct t2.
-
-  compute.
-  fold plus.
-  assert (n = n0) as H2; auto.
-  assert (n1 = n2) as H3; auto.
-  rewrite H2,H3.
-  omega.
-Qed.
-
-(*This is the diff function we developed in class 12/3*)
-
-Definition diff : forall A n (b : braun_tree A n) (m : nat) (P : m <= n <= m+1), nat .
-  refine (fun A => fix diff n (b : braun_tree A n) (m : nat) (P : m <= n <= m+1) : nat  :=
-            match b as b in braun_tree _ n with
-              |Empty => 0
-              |Node _ s1_size t1_size _ s1 t1 => 
-               match m with
-                 |0 => 1
-                 |S m'  => 
-                  match even_odd_dec m with
-                    |right H => 
-                     let k := (div2 (m - 1)) in
-                     diff s1_size s1 k _
-                    |left H =>
-                     let k := (div2 (m - 2)) in
-                     diff t1_size t1 k _
-                  end
-               end
-            end).
-inversion b.
