Makefile
@@ -1,25 +1,19 @@
 CPDTSRC = cpdt-src
 COQC = coqc
-GEN_DEPS = braun.vo util.vo
+GEN_DEPS = braun.vo util.vo monad.vo fl_log.vo
+# fl_log.vo here is more than strictly neccessary,
+# because make_array is probably not going to depend on it
 
-all: same_structure.vo insert.vo copy.vo counting_insert.vo counting_copy.vo
-
-construction: insert_time_by_construction.vo copy_time_by_construction.vo counting_make_array.vo monad2.vo
-
-same_structure.vo: same_structure.v $(GEN_DEPS)
-	$(COQC) same_structure.v
+all: insert.vo copy.vo size.vo
 
 insert.vo : insert.v $(GEN_DEPS)
 	$(COQC) insert.v
 
-counting_insert.vo : counting_insert.v monad.vo $(GEN_DEPS)
-	$(COQC) counting_insert.v
-
 copy.vo: copy.v $(GEN_DEPS)
 	$(COQC) copy.v
 
-counting_copy.vo : counting_copy.v monad.vo $(GEN_DEPS)
-	$(COQC) counting_copy.v
+size.vo: copy.v $(GEN_DEPS)
+	$(COQC) size.v
 
 braun.vo: braun.v
 	$(COQC) braun.v
@@ -29,21 +23,6 @@ util.vo: util.v
 
 monad.vo: monad.v util.vo
 	$(COQC) monad.v
-
-size_time_by_construction.vo: size_time_by_construction.v monad2.vo $(GEN_DEPS)
-	$(COQC) size_time_by_construction.v
-
-insert_time_by_construction.vo: insert_time_by_construction.v monad2.vo fl_log.vo $(GEN_DEPS)
-	$(COQC) insert_time_by_construction.v
-
-copy_time_by_construction.vo: copy_time_by_construction.v monad2.vo fl_log.vo $(GEN_DEPS)
-	$(COQC) copy_time_by_construction.v
-
-counting_make_array.vo: counting_make_array.v monad2.vo fl_log.vo braun.vo
-	$(COQC) counting_make_array.v
-
-monad2.vo: monad2.v util.vo
-	$(COQC) monad2.v
 
 fl_log.vo: fl_log.v util.vo
 	$(COQC) fl_log.v
